approx

src/tree_of_strategy.lean
@@ -72,6 +72,9 @@ lemma out_eq_iff {n} : ∀ {η : Tree n} {μ : branch η} {ν}, out μ = ν ↔ 
              { exfalso, simp at C, rcases C with ⟨_, rfl⟩, simp at this, exact this },
              { exact C } } } }
 
+lemma suffix_out_cons {n} {η : Tree n} (μ : branch η) : out μ :: μ.val <:+ η :=
+by { have := @out_eq_iff n η μ (out μ), simp* at* }
+
 lemma out_cons'_eq {n} {η : Tree n} (ν) (μ : branch η)  :
   @out n (ν :: η) μ.cons' = out μ :=
 by { simp[out, branch.cons'], intros h, exfalso, have := h μ.property, exact this }
@@ -82,63 +85,191 @@ def weight (μ : Tree 1) : Π {η : Tree 0} (υ : branch η → option (Tree 1))
 | []       _ := 0
 | (_ :: η) υ := @weight η (λ ν, υ ν.cons') + (if υ ⟨η, by simp⟩ = ↑μ then 1 else 0)
 
+lemma of_weight_pos {μ : Tree 1} : ∀ {η : Tree 0}
+  (υ : branch η → option (Tree 1)) (pos : 0 < weight μ υ), ∃ η₀ : branch η, υ η₀ = μ
+| []       υ pos := by { exfalso, simp[weight] at pos, exact pos }
+| (ν :: η) υ pos := by { 
+    by_cases C : υ ⟨η, by simp⟩ = ↑μ; simp[C, weight] at pos,
+    { refine ⟨⟨η, by simp⟩, C⟩ },
+    { rcases @of_weight_pos η (λ ν, υ ν.cons') pos with ⟨η₀, η₀_h⟩,
+      refine ⟨η₀.cons', η₀_h⟩ } }
+
+lemma weight_pos_of {μ : Tree 1} : ∀ {η : Tree 0}
+  (υ : branch η → option (Tree 1)) (h : ∃ η₀ : branch η, υ η₀ = μ), 0 < weight μ υ
+| [] _ h := by { exfalso, rcases h with ⟨⟨_, h⟩, _⟩, simp at h, exact h }
+| (ν :: η) υ h := by
+    { rcases h with ⟨η₀, h⟩,
+      have : η₀.val = η ∨ η₀.val ⊂ᵢ η, from list.is_initial_cons_iff.mp η₀.property,
+      cases this,
+      { simp[weight, ←this, h] },
+      { simp[weight], have := @weight_pos_of η (λ ν, υ ν.cons') ⟨⟨η₀.val, this⟩, by simp[branch.cons', h]⟩,
+        exact nat.add_pos_left this _ } }
+
 def is_exists_inv_infinity (μ : Tree 1) :
-  Π {η : Tree 0} (υ : branch η → option (Tree 1)), option (Tree 0)
+  Π {η : Tree 0} (υ : branch η → option (Tree 1)), option (branch η)
 | []               _ := none
 | (sum.inl _ :: η) υ :=
     if (@is_exists_inv_infinity η (λ ν, υ ν.cons')).is_some then
-      @is_exists_inv_infinity η (λ ν, υ ν.cons') else
-    if υ ⟨η, by simp⟩ = ↑μ then some η else none
-| (sum.inr _ :: η) υ := @is_exists_inv_infinity η (λ ν, υ ν.cons')
+      (@is_exists_inv_infinity η (λ ν, υ ν.cons')).map branch.cons' else
+    if υ ⟨η, by simp⟩ = ↑μ then some ⟨η, by simp⟩ else none
+| (sum.inr _ :: η) υ := (@is_exists_inv_infinity η (λ ν, υ ν.cons')).map branch.cons'
 
-lemma is_exists_inv_infinity_infinity
-  (η : Tree 1) {μ : Tree 0} (υ : branch μ → option (Tree 1)) (μ₀ : branch μ)
-  (h1 : out μ₀ = ∞) (h2 : υ μ₀ = η) : (is_exists_inv_infinity η υ).is_some :=
-begin
-  induction μ with ν μ IH μ IH generalizing μ₀,
-  { exfalso, have := μ₀.property, simp* at* },
-  have C₁ : μ₀.val = μ ∨ μ₀.val ⊂ᵢ μ, from list.is_initial_cons_iff.mp μ₀.property, cases C₁,
-  { cases ν; simp[is_exists_inv_infinity] at*,
-    { cases ν,
-      cases C₂ : (@is_exists_inv_infinity η μ (λ ν, υ ν.cons')).is_some; simp[C₂],
-      { simp[←C₁, h2] } },
-    { exfalso, have := out_eq_iff.mp h1, simp[←C₁] at this, exact this } },
-  { have IH : (is_exists_inv_infinity η (λ ν, υ ν.cons')).is_some,
-      from IH (λ ν, υ ν.cons') ⟨μ₀.val, C₁⟩
+lemma is_some_of_out_infinity {η : Tree 1} :
+  ∀ {μ : Tree 0} (υ : branch μ → option (Tree 1)) (μ₀ : branch μ)
+  (h1 : out μ₀ = ∞) (h2 : υ μ₀ = η), (is_exists_inv_infinity η υ).is_some 
+| []       υ μ₀ _  _  := by { exfalso, have := μ₀.property, simp* at*  }
+| (ν :: μ) υ μ₀ h1 h2 :=
+    begin
+      have C₁ : μ₀.val = μ ∨ μ₀.val ⊂ᵢ μ, from list.is_initial_cons_iff.mp μ₀.property, cases C₁,
+      { cases ν; simp[is_exists_inv_infinity] at*,
+        { cases ν,
+          cases C₂ : (@is_exists_inv_infinity η μ (λ ν, υ ν.cons')).is_some; simp[C₂],
+          { simp[←C₁, h2] },
+          { rcases option.is_some_iff_exists.mp C₂ with ⟨_, C₂⟩, simp[C₂] } },
+        { exfalso, have := out_eq_iff.mp h1, simp[←C₁] at this, exact this } },
+      { have IH : (is_exists_inv_infinity η (λ ν, υ ν.cons')).is_some,
+          from @is_some_of_out_infinity μ (λ ν, υ ν.cons') ⟨μ₀.val, C₁⟩
         (by {rw ←out_cons'_eq ν ⟨μ₀.val, C₁⟩, simp[branch.cons', h1] })
         (by simp[branch.cons', h2]),
-    cases ν; simp[is_exists_inv_infinity] at*; simp[IH] }
-end
+        cases ν; simp[is_exists_inv_infinity] at*; 
+        rcases option.is_some_iff_exists.mp IH with ⟨_, IH⟩; simp[IH] }
+    end
 
-lemma is_exists_inv_infinity_infinity'
-  (η : Tree 1) {μ : Tree 0} (υ : branch μ → option (Tree 1)) (μ₀ : branch μ)
-  (h : is_exists_inv_infinity η υ = some μ₀.val) : out μ₀ = ∞ ∧ υ μ₀ = η :=
+lemma out_infinity_of_eq_some {η : Tree 1} :
+  ∀ {μ : Tree 0} (υ : branch μ → option (Tree 1)) {μ₀ : branch μ}
+  (h : is_exists_inv_infinity η υ = some μ₀), out μ₀ = ∞ ∧ υ μ₀ = η
+| []               _ μ₀ _ := by { exfalso, have := μ₀.property, simp* at* }
+| (∞ :: μ)        υ μ₀ h :=
+    begin
+      cases C₁ : (@is_exists_inv_infinity η μ (λ ν, υ ν.cons')).is_some;
+      simp[is_exists_inv_infinity, C₁] at h,
+      { by_cases C₂ : υ ⟨μ, by simp⟩ = ↑η,
+        { simp[C₂] at h,
+          rcases h with rfl, simp[out_eq_iff, C₂] },
+        { exfalso, simp[C₂] at h, exact h } },
+      { rcases h with ⟨μ₁, h, eqn⟩,
+        have IH : out μ₁ = ∞ ∧ υ μ₁.cons' = ↑η,
+          from @out_infinity_of_eq_some _ (λ ν, υ ν.cons') μ₁ h,
+        simp[←eqn, out_cons'_eq], exact IH }
+    end
+| (sum.inr ν :: μ) υ μ₀ h :=
+    begin
+      simp[is_exists_inv_infinity] at h,
+      rcases h with ⟨μ₁, h, eqn⟩,
+        have IH : out μ₁ = ∞ ∧ υ μ₁.cons' = ↑η,
+          from @out_infinity_of_eq_some _ (λ ν, υ ν.cons') μ₁ h,
+      simp[←eqn, out_cons'_eq], exact IH
+    end
+
+lemma out_neq_infinity_of_eq_none {η : Tree 1}
+  {μ : Tree 0} (υ : branch μ → option (Tree 1))
+  (h : is_exists_inv_infinity η υ = none) (μ₀ : branch μ) : υ μ₀ = η → out μ₀ ≠ ∞ :=
 begin
-  induction μ with ν μ IH μ IH generalizing μ₀,
-  { exfalso, have := μ₀.property, simp* at* },
-  have C₁ : μ₀.val = μ ∨ μ₀.val ⊂ᵢ μ, from list.is_initial_cons_iff.mp μ₀.property, cases C₁,
-  { have : μ₀ = ⟨μ, by simp⟩, { apply subtype.ext, exact C₁ },
-    rcases this with rfl, 
-    cases ν; simp[is_exists_inv_infinity] at*,
-    { cases ν,
-      cases C₂ : (@is_exists_inv_infinity η μ (λ ν, υ ν.cons')).is_some; simp[C₂] at h,
-      { simp[out_eq_iff], exact classical.by_contradiction h },
-      { exfalso,   } } }
-
+  by_cases C : υ μ₀ = ↑η ∧ out μ₀ = ∞,
+  { exfalso, have := is_some_of_out_infinity υ μ₀ C.2 C.1, simp[h] at this, exact this },
+  { simp at C, exact C }
 end
+
+lemma eq_none_of_out_neq_infinity {η : Tree 1} :
+  ∀ {μ : Tree 0} (υ : branch μ → option (Tree 1))
+  (h : ∀ μ₀ : branch μ, υ μ₀ = η → out μ₀ ≠ ∞), is_exists_inv_infinity η υ = none
+| []       _ _ := by simp[is_exists_inv_infinity]
+| (ν :: μ) υ h :=
+    begin
+      have : ∀ (μ₀ : branch μ), υ μ₀.cons' = ↑η → out μ₀ ≠ ∞,
+        { intros μ₀, simp[←out_cons'_eq ν μ₀, branch.cons'],
+          have := h ⟨μ₀.val, μ₀.property.trans (μ.is_initial_cons _)⟩, exact this }, 
+        have : is_exists_inv_infinity η (λ ν, υ ν.cons') = none,
+          from eq_none_of_out_neq_infinity (λ ν, υ ν.cons') this,
+        cases ν; simp[is_exists_inv_infinity, this],
+        { cases ν, intros hμ,
+          have : out ⟨μ, _⟩ ≠ ∞ := h ⟨μ, by simp⟩ hμ,
+          simp[out_eq_iff] at this, exact this }
+    end
 
 def lambda' {η : Tree 0} (υ : branch η → option (Tree 1)) : ℕ → Tree 1
 | 0       := []
 | (n + 1) :=
     if 0 < weight (lambda' n) υ then
       if h : (is_exists_inv_infinity (lambda' n) υ).is_some then
-        sum.inr (option.get h) :: lambda' n
+        sum.inr (option.get h).val :: lambda' n
       else ∞ :: lambda' n
     else lambda' n
 
+lemma lambda'_suffix_eq {η : Tree 0} (υ : branch η → option (Tree 1)) : ∀ {n : ℕ}
+  {x} {μ : Tree 1} (hμ : x :: μ <:+ lambda' υ n),
+  ∃ m, m < n ∧ lambda' υ m = μ ∧ lambda' υ (m + 1) = x :: μ
+| 0       x μ h := by { exfalso, simp[lambda', *] at * }
+| (n + 1) x μ h :=
+    begin
+      simp[lambda'] at h,
+      by_cases C₁ : 0 < weight (lambda' υ n) υ; simp[C₁] at h,
+      { cases C₂ : (is_exists_inv_infinity (lambda' υ n) υ).is_some; simp[C₂] at h,
+        { have C₃ : x :: μ = ∞ :: lambda' υ n ∨ x :: μ <:+ lambda' υ n, from list.suffix_cons_iff.mp h,
+          cases C₃,
+          { simp at C₃, refine ⟨n, lt_add_one n, by simp[C₃], by simp[lambda', C₁, C₂, C₃]⟩ },
+          { rcases @lambda'_suffix_eq n x μ C₃ with ⟨m, IH₁, IH₂⟩,
+            refine ⟨m, nat.lt.step IH₁, IH₂⟩ } },
+        { have C₃ : x :: μ = sum.inr (option.get C₂).val :: lambda' υ n ∨ x :: μ <:+ lambda' υ n,
+            from list.suffix_cons_iff.mp h,
+          cases C₃,
+          { simp at C₃, refine ⟨n, lt_add_one n, by simp[C₃], by simp[lambda', C₁, C₂, C₃]⟩ },
+          { rcases @lambda'_suffix_eq n x μ C₃ with ⟨m, IH₁, IH₂⟩,
+            refine ⟨m, nat.lt.step IH₁, IH₂⟩ } } },
+      rcases @lambda'_suffix_eq n x μ h with ⟨m, IH₁, IH₂⟩,
+      refine ⟨m, nat.lt.step IH₁, IH₂⟩
+    end
+
+lemma out_infinity_of_out_inr {η : Tree 0} (υ : branch η → option (Tree 1)) {n : ℕ}
+  {μ : branch (lambda' υ n)} {η₀ : Tree 0} (h : out μ = sum.inr η₀) :
+  ∃ h : η₀ ⊂ᵢ η, out ⟨η₀, h⟩ = ∞ ∧ υ ⟨η₀, h⟩ = μ.val :=
+begin
+  have : ∃ m, m < n ∧ lambda' υ m = μ.val ∧ lambda' υ (m + 1) = sum.inr η₀ :: μ.val,
+  { simp[out_eq_iff] at h, refine lambda'_suffix_eq υ h },
+  rcases this with ⟨m, eqn_m, eqn_μ, eqn_μ'⟩,
+  by_cases C₁ : 0 < weight (lambda' υ m) υ; simp[lambda', C₁] at eqn_μ',
+  { cases C₂ : is_exists_inv_infinity (lambda' υ m) υ with ν; simp[C₂] at eqn_μ',
+    { exfalso, have := list.head_eq_of_cons_eq eqn_μ', simp* at * },
+    { have : ν.val = η₀,
+        from sum.inr.inj (list.head_eq_of_cons_eq eqn_μ'),
+      rcases this with rfl,
+      refine ⟨ν.property, _⟩, simp,
+      have : out ν = ∞ ∧ υ ν = ↑(lambda' υ m), from out_infinity_of_eq_some υ C₂,
+      simp[eqn_μ, this] at* } },
+  exfalso, simp[eqn_μ] at eqn_μ', exact eqn_μ'
+end
+
+lemma out_infinity_of_out_neq_infinity
+  {η : Tree 0} (υ : branch η → option (Tree 1)) {n : ℕ} {μ : branch (lambda' υ n)}
+  (h₁ : ∃ η₀ : branch η, υ η₀ = μ.val) (h₂ : ∀ η₀ : branch η, υ η₀ = μ.val → out η₀ ≠ ∞) :
+  out μ = ∞ :=
+begin
+  have : ∃ m, m < n ∧ lambda' υ m = μ.val ∧ lambda' υ (m + 1) = out μ :: μ.val,
+    from lambda'_suffix_eq υ (suffix_out_cons μ),
+  rcases this with ⟨m, eqn_m, eqn_μ, eqn_μ'⟩,
+  have lmm₁ : 0 < weight μ.val υ, from weight_pos_of υ h₁,
+  have lmm₂ : is_exists_inv_infinity μ.val υ = none, from eq_none_of_out_neq_infinity υ h₂, simp at*,
+  simp[lambda', eqn_μ, lmm₁, lmm₂] at eqn_μ',
+  exact eq.symm (list.head_eq_of_cons_eq eqn_μ')
+end
+
+lemma out_neq_infinity_of_out_infinity {η : Tree 0} (υ : branch η → option (Tree 1)) {n : ℕ}
+  {μ : branch (lambda' υ n)} (h : out μ = ∞) :
+  (∃ η₀ : branch η, υ η₀ = μ.val) ∧ (∀ η₀ : branch η, υ η₀ = μ.val → out η₀ ≠ ∞) :=
+begin
+  have : ∃ m, m < n ∧ lambda' υ m = μ.val ∧ lambda' υ (m + 1) = ∞ :: μ.val,
+  { simp[out_eq_iff] at h, exact lambda'_suffix_eq υ h },
+  rcases this with ⟨m, eqn_m, eqn_μ, eqn_μ'⟩,
+  by_cases C₁ : 0 < weight (lambda' υ m) υ; simp[lambda', C₁] at eqn_μ',
+  { cases C₂ : is_exists_inv_infinity (lambda' υ m) υ with ν; simp[C₂] at eqn_μ',
+    { simp[←eqn_μ], refine ⟨of_weight_pos υ C₁, out_neq_infinity_of_eq_none υ C₂⟩ },
+    { exfalso, have := list.head_eq_of_cons_eq eqn_μ', simp* at* } },
+  { exfalso, simp[eqn_μ] at eqn_μ', exact eqn_μ' }
+end
+
 def lambda {η : Tree 0} (υ : branch η → option (Tree 1)) : Tree 1 := lambda' υ η.length
 
-def assign {η : Tree 0} (υ : branch η → option (Tree 1)) : Tree 1 → option (Tree 1 × ℕ)
+def assign {η : Tree 0} (υ : branch η → option (Tree 1)) : Π μ : Tree 1, option (Tree 1 × ℕ)
 | []               := none
 | (∞ :: μ)        :=
   if h : (assign μ).is_some then S.inf (option.get h) (μ, weight μ υ) else
@@ -179,14 +310,10 @@ def assignment (η : Tree 0) : option (Tree 1 × ℕ) := approx.assignment S (up
 
 @[simp] lemma lambda_nil : S.lambda [] = [] := rfl
 
-lemma is_exists_inv_infinity_infinity (μ : Tree 0) (μ₀ : branch μ) (η : branch (S.lambda μ)) 
-  (h1 : out μ₀ = ∞) (h2 : S.up μ₀.val = η.val) : out η = sum.inr μ₀.val :=
-begin
-  induction μ with ν μ IH μ IH generalizing μ₀; simp[out] at*,
-  { exfalso, have := μ₀.property, simp* at* },
-  simp[lambda, approx.lambda],
-end
-
+lemma out_neq_infinity_of_out_infinity {η : Tree 0} {μ : branch (S.lambda η)}
+  (h : out μ = ∞) {η₀ : branch η} (up : S.up η₀.val = μ.val) : out η₀ ≠ ∞ :=
+(approx.out_neq_infinity_of_out_infinity (up' S η) h).2 η₀
+(by { simp[up'_up_consistent], exact up })
 
 variables (Λ : Tree_path 0)
 
